remove bedrock from COQ_ARGS because we all use COQPATH
BoundedWord2

Factor out a tactic and add more examples

BoundedWord2: add test cases

intermediate stage

simple

src/Assembly/BoundedWord.v
@@ -1,6 +1,6 @@
 
-Require Import Bedrock.Word.
-Require Import NArith PArith Ndigits Compare_dec.
+Require Import Bedrock.Word Bedrock.Nomega.
+Require Import NArith PArith Ndigits Compare_dec Arith.
 Require Import ProofIrrelevance.
 Require Import Ring.
 
@@ -10,18 +10,394 @@ Section BoundedWord.
 
   Open Scope Bounded_scope.
 
-  (* First, we make our BoundedWord sigma type *)
-  Definition wordGeN {n: nat} (a: word n) (b: N): Prop :=
-    (wordToN a >= b)%N.
+  Variable n: nat.
 
+  (* Word Operations *)
+
+  Definition shiftr (w: word n) (bits: nat): word n.
+    destruct (le_dec bits n).
+
+    - replace n with (bits + (n - bits)) in * by (abstract intuition).
+      refine (zext (split1 bits (n - bits) w) (n - bits)).
+
+    - exact (wzero n).
+  Defined.
+
+  Lemma shiftr_spec: forall (w : word n) (bits: nat),
+      wordToN (shiftr w bits) = N.shiftr (wordToN w) (N.of_nat bits).
+    intros; unfold shiftr; destruct (le_dec bits n).
+
+    - admit.
+
+    - replace (wordToN (wzero n)) with 0%N by admit.
+      unfold N.shiftr.
+      induction bits.
+
+      + replace (N.of_nat 0) with 0%N by intuition.
+        assert (n = 0) by intuition; clear n0; subst.
+        replace w with WO; intuition.
+
+      + induction bits; admit.
+  Qed.
+
+  Definition mask (m: nat) (w: word n): word n.
+    destruct (le_dec m n).
+
+    - replace n with (m + (n - m)) in * by (abstract intuition).
+      refine (w ^& (zext (wones m) (n - m))).
+
+    - exact w.
+  Defined.
+
+  (* Definitions of Inequality and simple bounds. *)
   Definition wordLeN {n: nat} (a: word n) (b: N): Prop :=
     (wordToN a <= b)%N.
 
-  Notation "A >= B" := (wordGeN A B) (at level 70) : Bounded_scope.
   Notation "A <= B" := (wordLeN A B) (at level 70) : Bounded_scope.
 
-  Inductive BoundOn {n: nat} (x: word n) : Prop :=
-    | boundBy: forall low high: N, x >= low -> x <= high -> BoundOn x.
+  Lemma le_ge : forall n m, (n <= m -> m >= n)%nat.
+  Proof.
+    intros; omega.
+  Qed.
+
+  Lemma ge_le : forall n m, (n >= m -> m <= n)%nat.
+  Proof.
+    intros; omega.
+  Qed.
+
+  Ltac ge_to_le :=
+    try apply N.ge_le;
+    repeat match goal with
+           | [ H : _ |- _ ] => apply N.le_ge in H
+           end.
+
+  Ltac ge_to_le_nat :=
+    try apply le_ge;
+    repeat match goal with
+           | [ H : _ |- _ ] => apply ge_le in H
+           end.
+
+  Ltac preomega := unfold wordLeN; intros; ge_to_le; pre_nomega.
+
+  Hint Rewrite wordToN_nat Nat2N.inj_add N2Nat.inj_add Nat2N.inj_mul N2Nat.inj_mul Npow2_nat : N.
+
+  Theorem word_size_bound : forall (w: word n),
+    w <= Npow2 n - 1.
+  Proof.
+    intros; unfold wordLeN; rewrite wordToN_nat.
+
+    assert (B := wordToNat_bound w);
+      rewrite <- Npow2_nat in B;
+      apply nat_compare_lt in B.
+
+    unfold N.le; intuition;
+      rewrite N2Nat.inj_compare in H;
+      rewrite Nat2N.id in H.
+
+    apply nat_compare_lt in B.
+    apply nat_compare_gt in H.
+
+    replace (N.to_nat (Npow2 n)) with (S (N.to_nat (Npow2 n - 1))) in * by admit.
+    intuition.
+  Qed.
+
+  Theorem constant_bound_N : forall k,
+    NToWord n k <= k.
+  Proof.
+    preomega.
+    rewrite NToWord_nat.
+    destruct (le_lt_dec (pow2 n) (N.to_nat k)).
+
+    specialize (wordToNat_bound (natToWord n (N.to_nat k))); nomega.
+
+    rewrite wordToNat_natToWord_idempotent; nomega.
+  Qed.
+
+  Theorem constant_bound_nat : forall k,
+    natToWord n k <= N.of_nat k.
+  Proof.
+    preomega.
+    destruct (le_lt_dec (pow2 n) k).
+
+    specialize (wordToNat_bound (natToWord n k)); nomega.
+
+    rewrite wordToNat_natToWord_idempotent; nomega.
+  Qed.
+
+  Theorem wplus_bound : forall (w1 w2 : word n) b1 b2,
+    w1 <= b1
+    -> w2 <= b2
+    -> w1 ^+ w2 <= b1 + b2.
+  Proof.
+    preomega.
+    destruct (le_lt_dec (pow2 n) (N.to_nat b1 + N.to_nat b2)).
+
+    specialize (wordToNat_bound (w1 ^+ w2)); nomega.
+
+    rewrite wplus_alt.
+    unfold wplusN, wordBinN.
+    rewrite wordToNat_natToWord_idempotent; nomega.
+  Qed.
+
+  Theorem wmult_bound : forall (w1 w2 : word n) b1 b2,
+    w1 <= b1
+    -> w2 <= b2
+    -> w1 ^* w2 <= b1 * b2.
+  Proof.
+    preomega.
+    destruct (le_lt_dec (pow2 n) (N.to_nat b1 * N.to_nat b2)).
+
+    specialize (wordToNat_bound (w1 ^* w2)); nomega.
+
+    rewrite wmult_alt.
+    unfold wmultN, wordBinN.
+    rewrite wordToNat_natToWord_idempotent.
+    ge_to_le_nat.
+
+    apply Mult.mult_le_compat; nomega.
+    pre_nomega.
+    apply Lt.le_lt_trans with (N.to_nat b1 * N.to_nat b2); auto.
+    apply Mult.mult_le_compat; nomega.
+  Qed.
+
+  Theorem shiftr_bound : forall (w : word n) b bits,
+    w <= b
+    -> shiftr w bits <= N.shiftr b (N.of_nat bits).
+  Proof.
+    admit.
+  Qed.
+
+  Theorem mask_bound : forall (w : word n) m,
+    mask m w <= Npow2 m - 1.
+  Proof.
+    admit.
+  Qed.
+
+  Theorem mask_update_bound : forall (w : word n) b m,
+    w <= b
+    -> mask m w <= (N.min b (Npow2 m - 1)).
+  Proof.
+    admit.
+  Qed.
+
+
+  Ltac word_bound :=
+    repeat (
+       eassumption
+       || apply wplus_bound
+       || apply wmult_bound
+       || apply mask_update_bound
+       || apply mask_bound
+       || apply shiftr_bound
+       || apply constant_bound_N
+       || apply constant_bound_nat
+       || apply word_size_bound
+      ).
+
+  Notation "$" := (natToWord _).
+
+  Lemma example1 : forall (w1 w2 w3 w4 : word n) b1 b2 b3 b4,
+    w1 <= b1
+    -> w2 <= b2
+    -> w3 <= b3
+    -> w4 <= b4
+    -> { b | w1 ^+ (w2 ^* w3) ^* w4 <= b }.    
+  Proof.
+    eexists.
+    word_bound.
+  Defined.
+
+  (* Eval simpl in fun (w1 w2 w3 w4 : word n) (b1 b2 b3 b4 : N)
+                    (H1 : w1 <= b1) (H2 : w2 <= b2) (H3 : w3 <= b3) (H4 : w4 <= b4) =>
+                  projT1 (example1 H1 H2 H3 H4). *)
+
+  Lemma example2 : forall (w1 w2 w3 w4 : word n) b1 b2 b3 b4,
+    w1 <= b1
+    -> w2 <= b2
+    -> w3 <= b3
+    -> w4 <= b4
+    -> { b | w1 ^+ (w2 ^* $7 ^* w3) ^* w4 ^+ $8 ^+ w2 <= b }.
+  Proof.
+    eexists.
+    word_bound.
+  Defined.
+
+  (*Eval simpl in fun (w1 w2 w3 w4 : word n) (b1 b2 b3 b4 : N)
+                    (H1 : w1 <= b1) (H2 : w2 <= b2) (H3 : w3 <= b3) (H4 : w4 <= b4) =>
+                  projT1 (example2 H1 H2 H3 H4). *)
+
+  Lemma example3 : forall (w1 w2 w3 w4 : word n),
+    w1 <= Npow2 3
+    -> w2 <= Npow2 4
+    -> w3 <= Npow2 8
+    -> w4 <= Npow2 16
+    -> { b | w1 ^+ (w2 ^* $7 ^* w3) ^* w4 ^+ $8 ^+ w2 <= b }.
+  Proof.
+    eexists.
+    word_bound.
+  Defined.
+
+  (* Eval simpl in fun (w1 w2 w3 w4 : word n)
+                    (H1 : w1 <= _) (H2 : w2 <= _) (H3 : w3 <= _) (H4 : w4 <= _) =>
+                  projT1 (example3 H1 H2 H3 H4). *)
+
+End BoundedWord.
+
+Section MulmodExamples.
+
+  Notation "A <= B" := (wordLeN A B) (at level 70).
+  Notation "$" := (natToWord _).
+
+  Ltac word_bound :=
+    repeat (
+       eassumption
+       || apply (wplus_bound 32)
+       || apply (wmult_bound 32)
+       || apply (mask_update_bound 32)
+       || apply (mask_bound 32)
+       || apply (shiftr_bound 32)
+       || apply (constant_bound_N 32)
+       || apply (constant_bound_nat 32)
+       || apply (word_size_bound 32)
+      ).
+
+  Lemma example_and : forall x : word 32, wand x (NToWord 32 (N.ones 10)) <= 1023.
+    intros.
+    replace (wand x (NToWord 32 (N.ones 10))) with (mask 32 10 x) by admit.
+    word_bound.
+  Qed.
+    
+  Lemma example_shiftr : forall x : word 32, shiftr 32 x 30 <= 3.
+    intros.
+    replace 3%N with (N.shiftr (Npow2 32 - 1) (N.of_nat 30)) by (simpl; intuition).
+
+    (* word_bound works but it's slow *)
+    apply (shiftr_bound 32).
+    apply (word_size_bound 32).
+  Qed.
+
+  Lemma example_shiftr2 : forall x : word 32, x <= 1023 -> shiftr 32 x 5 <= 31.
+    intros.
+    replace 31%N with (N.shiftr 1023%N 5%N) by (simpl; intuition).
+
+    (* word_bound works but it's slow *)
+    apply (shiftr_bound 32).
+    eassumption.
+  Qed.
+    
+  Variable f0 f1 f2 f3 f4 f5 f6 f7 f8 f9 : word 32.
+  Variable g0 g1 g2 g3 g4 g5 g6 g7 g8 g9 : word 32.
+  Hypothesis Hf0 : f0 <= 2^26.
+  Hypothesis Hf1 : f1 <= 2^25.
+  Hypothesis Hf2 : f2 <= 2^26.
+  Hypothesis Hf3 : f3 <= 2^25.
+  Hypothesis Hf4 : f4 <= 2^26.
+  Hypothesis Hf5 : f5 <= 2^25.
+  Hypothesis Hf6 : f6 <= 2^26.
+  Hypothesis Hf7 : f7 <= 2^25.
+  Hypothesis Hf8 : f8 <= 2^26.
+  Hypothesis Hf9 : f9 <= 2^25.
+  Hypothesis Hg0 : g0 <= 2^26.
+  Hypothesis Hg1 : g1 <= 2^25.
+  Hypothesis Hg2 : g2 <= 2^26.
+  Hypothesis Hg3 : g3 <= 2^25.
+  Hypothesis Hg4 : g4 <= 2^26.
+  Hypothesis Hg5 : g5 <= 2^25.
+  Hypothesis Hg6 : g6 <= 2^26.
+  Hypothesis Hg7 : g7 <= 2^25.
+  Hypothesis Hg8 : g8 <= 2^26.
+  Hypothesis Hg9 : g9 <= 2^25.
+    
+  Lemma example_mulmod_s_ppt : { b | f0 ^* g0  <= b}.
+    eexists.
+    word_bound.
+  Defined.
+
+  Lemma example_mulmod_s_pp :  { b | f0 ^* g0 ^+ $19 ^* (f9 ^* g1 ^* $2 ^+ f8 ^* g2 ^+ f7 ^* g3 ^* $2 ^+ f6 ^* g4 ^+ f5 ^* g5 ^* $2 ^+ f4 ^* g6 ^+ f3 ^* g7 ^* $2 ^+ f2 ^* g8 ^+  f1 ^* g9 ^* $2) <= b}.
+    eexists.
+    word_bound.
+  Defined.
+
+  Lemma example_mulmod_s_pp_shiftr :
+      { b | shiftr (f0 ^* g0 ^+  $19 ^* (f9 ^* g1 ^* $2 ^+ f8 ^* g2 ^+ f7 ^* g3 ^* $2 ^+ f6 ^* g4 ^+ f5 ^* g5 ^* $2 ^+ f4 ^* g6 ^+ f3 ^* g7 ^* $2 ^+ f2 ^* g8 ^+  f1 ^* g9 ^* $2)) 26 <= b}.
+    eexists.
+    word_bound.
+  Qed.
+
+  Lemma example_mulmod_u_fg1 :  { b |
+        (let y : word 32 := (* the type declarations on the let-s make type inference not take forever *)
+           (f0 ^* g0 ^+
+            $19 ^*
+            (f9 ^* g1 ^* $2 ^+ f8 ^* g2 ^+ f7 ^* g3 ^* $2 ^+ f6 ^* g4 ^+ f5 ^* g5 ^* $2 ^+ f4 ^* g6 ^+ f3 ^* g7 ^* $2 ^+ f2 ^* g8 ^+
+             f1 ^* g9 ^* $2)) in
+         let y0 : word 32 :=
+           (shiftr y 26 ^+
+            (f1 ^* g0 ^+ f0 ^* g1 ^+
+             $19 ^* (f9 ^* g2 ^+ f8 ^* g3 ^+ f7 ^* g4 ^+ f6 ^* g5 ^+ f5 ^* g6 ^+ f4 ^* g7 ^+ f3 ^* g8 ^+ f2 ^* g9))) in
+         let y1 : word 32 :=
+           (shiftr y0 25 ^+
+            (f2 ^* g0 ^+ f1 ^* g1 ^* $2 ^+ f0 ^* g2 ^+
+             $19 ^* (f9 ^* g3 ^* $2 ^+ f8 ^* g4 ^+ f7 ^* g5 ^* $2 ^+ f6 ^* g6 ^+ f5 ^* g7 ^* $2 ^+ f4 ^* g8 ^+ f3 ^* g9 ^* $2))) in
+         let y2 : word 32 :=
+           (shiftr y1 26 ^+
+            (f3 ^* g0 ^+ f2 ^* g1 ^+ f1 ^* g2 ^+ f0 ^* g3 ^+
+             $19 ^* (f9 ^* g4 ^+ f8 ^* g5 ^+ f7 ^* g6 ^+ f6 ^* g7 ^+ f5 ^* g8 ^+ f4 ^* g9))) in
+         let y3 : word 32 :=
+           (shiftr y2 25 ^+
+            (f4 ^* g0 ^+ f3 ^* g1 ^* $2 ^+ f2 ^* g2 ^+ f1 ^* g3 ^* $2 ^+ f0 ^* g4 ^+
+             $19 ^* (f9 ^* g5 ^* $2 ^+ f8 ^* g6 ^+ f7 ^* g7 ^* $2 ^+ f6 ^* g8 ^+ f5 ^* g9 ^* $2))) in
+         let y4 : word 32 :=
+           (shiftr y3 26 ^+
+            (f5 ^* g0 ^+ f4 ^* g1 ^+ f3 ^* g2 ^+ f2 ^* g3 ^+ f1 ^* g4 ^+ f0 ^* g5 ^+
+             $19 ^* (f9 ^* g6 ^+ f8 ^* g7 ^+ f7 ^* g8 ^+ f6 ^* g9))) in
+         let y5 : word 32 :=
+           (shiftr y4 25 ^+
+            (f6 ^* g0 ^+ f5 ^* g1 ^* $2 ^+ f4 ^* g2 ^+ f3 ^* g3 ^* $2 ^+ f2 ^* g4 ^+ f1 ^* g5 ^* $2 ^+ f0 ^* g6 ^+
+             $19 ^* (f9 ^* g7 ^* $2 ^+ f8 ^* g8 ^+ f7 ^* g9 ^* $2))) in
+         let y6 : word 32 :=
+           (shiftr y5 26 ^+
+            (f7 ^* g0 ^+ f6 ^* g1 ^+ f5 ^* g2 ^+ f4 ^* g3 ^+ f3 ^* g4 ^+ f2 ^* g5 ^+ f1 ^* g6 ^+ f0 ^* g7 ^+
+             $19 ^* (f9 ^* g8 ^+ f8 ^* g9))) in
+         let y7 : word 32 :=
+           (shiftr y6 25 ^+
+            (f8 ^* g0 ^+ f7 ^* g1 ^* $2 ^+ f6 ^* g2 ^+ f5 ^* g3 ^* $2 ^+ f4 ^* g4 ^+ f3 ^* g5 ^* $2 ^+ f2 ^* g6 ^+ f1 ^* g7 ^* $2 ^+
+             f0 ^* g8 ^+ $19 ^* f9 ^* g9 ^* $2)) in
+         let y8 : word 32 :=
+           (shiftr y7 26 ^+
+            (f9 ^* g0 ^+ f8 ^* g1 ^+ f7 ^* g2 ^+ f6 ^* g3 ^+ f5 ^* g4 ^+ f4 ^* g5 ^+ f3 ^* g6 ^+ f2 ^* g7 ^+ f1 ^* g8 ^+
+             f0 ^* g9)) in
+         let y9 : word 32 :=
+           ($19 ^* shiftr y8 25 ^+
+            wand
+              (f0 ^* g0 ^+
+               $19 ^*
+               (f9 ^* g1 ^* $2 ^+ f8 ^* g2 ^+ f7 ^* g3 ^* $2 ^+ f6 ^* g4 ^+ f5 ^* g5 ^* $2 ^+ f4 ^* g6 ^+ f3 ^* g7 ^* $2 ^+
+                f2 ^* g8 ^+ f1 ^* g9 ^* $2)) (@NToWord 32 (N.ones 26%N))) in
+         let fg1 : word 32 := (shiftr y9 26 ^+
+          wand
+            (shiftr y 26 ^+
+             (f1 ^* g0 ^+ f0 ^* g1 ^+
+              $19 ^* (f9 ^* g2 ^+ f8 ^* g3 ^+ f7 ^* g4 ^+ f6 ^* g5 ^+ f5 ^* g6 ^+ f4 ^* g7 ^+ f3 ^* g8 ^+ f2 ^* g9)))
+            (@NToWord 32 (N.ones 26%N))) in
+         fg1) <= b }.
+  Abort.
+
+  Require Import ZArith.
+  Variable shiftra : forall {l}, word l -> nat -> word l. (* "arithmetic" aka "signed" bitshift *)
+  Hypothesis shiftra_spec : forall {l} (w : word l) (n:nat), wordToZ (shiftra w n) = Z.shiftr (wordToZ w) (Z.of_nat n).
+
+  Lemma example_shiftra : forall x : word 4, shiftra x 2 <= 15.
+  Abort.
+
+  Lemma example_shiftra : forall x : word 4, x <= 7 -> shiftra x 2 <= 1.
+  Abort.
+
+  Lemma example_mulmod_s_pp_shiftra :
+      { b | shiftra (f0 ^* g0 ^+  $19 ^* (f9 ^* g1 ^* $2 ^+ f8 ^* g2 ^+ f7 ^* g3 ^* $2 ^+ f6 ^* g4 ^+ f5 ^* g5 ^* $2 ^+ f4 ^* g6 ^+ f3 ^* g7 ^* $2 ^+ f2 ^* g8 ^+  f1 ^* g9 ^* $2)) 26 <= b}.
+  Abort.
+End MulmodExamples.
+
+(* Old lemmas that might end up being useful
 
   Lemma low_word_bound: forall n (x : word n), x >= 0.
     intros; unfold wordGeN;
@@ -96,7 +472,6 @@ Section BoundedWord.
     intros; apply proof_irrelevance.
   Qed.
 
-  (* Get inequalities from definitions *)
   Lemma wand_upper_l: forall (n: nat) (x a b: word n), x = wand a b -> x <= (2 * wordToN a)%N.
     admit.
   Qed.
@@ -152,7 +527,6 @@ Section BoundedWord.
       inversion H.
   Qed.
 
-  (* Essential operations on bounded words *)
   Definition bplus {n: nat} {x y: word n} (A: BoundOn x) (B: BoundOn y): BoundOn (wplus x y).
     destruct A as [low0 high0 lb0 hb0], B as [low1 high1 lb1 hb1].
 
@@ -165,22 +539,13 @@ Section BoundedWord.
     - apply (boundBy (x ^+ y) low0 high0); admit.
 
     - apply (boundBy (x ^+ y) (low0 + low1)%N (high0 + high1)%N); admit.
-      (* rewrite wplus_alt;
-         unfold wplusN, wordGeN, wordBinN in *; simpl;
-           rewrite wordToN_nat, wordToNat_natToWord_idempotent;
-           rewrite Nat2N.inj_add; repeat rewrite <- wordToN_nat.*)
   Defined.
 
   Definition bmult {n: nat} {x y: word n} (A: BoundOn x) (B: BoundOn y): BoundOn (wmult x y).
     destruct A as [low0 high0 lb0 hb0], B as [low1 high1 lb1 hb1].
     apply (boundBy (x ^* y) (low0 * low1)%N (high0 * high1)%N); admit.
-      (* rewrite wmult_alt;
-        unfold wmultN, wordLeN, wordBinN in *; simpl;
-        rewrite wordToN_nat, wordToNat_natToWord_idempotent;
-        rewrite Nat2N.inj_mul; repeat rewrite <- wordToN_nat. *)
   Defined.
 
-  (* Operation replacements *)
   Lemma bound_plus: forall (n: nat) (a b: word n), bound (wplus a b) = bplus (bound a) (bound b).
     intros; apply proof_irrelevance.
   Qed.
@@ -189,7 +554,6 @@ Section BoundedWord.
     intros; apply proof_irrelevance.
   Qed.
 
-  (* Tactics to repeatedly apply the simplification strategy *)
   Ltac convert_to_bounded :=
     apply bound_eq;
     repeat first [rewrite bound_plus | rewrite bound_mult].
@@ -209,14 +573,13 @@ Section BoundedWord.
       | [|- context[sumbool_ind _ _ _ (zero_dec ?x)]] => destruct (zero_dec x)
       end; subst).
 
-  (* Miscellaneous simplifications we'll need *)
   Ltac word_simpl :=
     repeat (
       match goal with
       | [|- context [unbound _]] => unfold unbound
-      (*| [ H: (Npow2 ?x = 0)%N |- _] =>
+      | [ H: (Npow2 ?x = 0)%N |- _] =>
         let Z := fresh in
-          apply (Npow2_nonzero x) in H; intuition *)
+          apply (Npow2_nonzero x) in H; intuition
       | [ H: (?x <= 0) |- _] =>
         unfold wordLeN in H;
         apply replace_zero in H;
@@ -230,15 +593,12 @@ Section BoundedWord.
            bound, bplus, bmult,
            wand_bound_l, wand_bound_r.
 
-  (* The full tactic *)
   Ltac bound_simpl:=
     convert_to_bounded;
     propagate_bounds;
     unfold_ops;
     repeat match_match;
     word_simpl.
-
-  (* Example Lemma *)
 
   Lemma example_bound_simpl: forall (n: nat) (a b: word n),
     a = wand (wzero n) b -> b = a ^+ b.
@@ -248,6 +608,4 @@ Section BoundedWord.
     propagate_bounds.
     unfold_ops; simpl.
     match_match; word_simpl.
-  Qed.
-
-End BoundedWord.
+  Qed. *)
